pollux/lib/pollux/Pollux_Proto_Parse.ml
@@ -7,6 +7,8 @@ let (nat_to_u32 : Prims.nat -> FStar_UInt32.t) =
 let (nat_to_u64 : Prims.nat -> FStar_UInt64.t) =
   fun n ->
     FStar_UInt64.uint_to_t (FStar_UInt.to_uint_t (Prims.of_int (64)) n)
+let (int_to_i32 : Prims.int -> FStar_Int32.t) =
+  fun z -> FStar_Int32.int_to_t (FStar_Int.to_int_t (Prims.of_int (32)) z)
 let (int_to_i64 : Prims.int -> FStar_Int64.t) =
   fun z -> FStar_Int64.int_to_t (FStar_Int.to_int_t (Prims.of_int (64)) z)
 let rec (exp : Prims.int -> Prims.nat -> Prims.int) =
@@ -126,29 +128,6 @@ let (tag_num : tag -> FStar_UInt64.t) =
     | I64 -> nat_to_u64 Prims.int_one
     | LEN -> nat_to_u64 (Prims.of_int (2))
     | I32 -> nat_to_u64 (Prims.of_int (5))
-let op_let_Question :
-  'a 'b .
-    'a FStar_Pervasives_Native.option ->
-      ('a -> 'b FStar_Pervasives_Native.option) ->
-        'b FStar_Pervasives_Native.option
-  =
-  fun x ->
-    fun f ->
-      match x with
-      | FStar_Pervasives_Native.Some x1 -> f x1
-      | FStar_Pervasives_Native.None -> FStar_Pervasives_Native.None
-let op_and_Question :
-  'a 'b .
-    'a FStar_Pervasives_Native.option ->
-      'b FStar_Pervasives_Native.option ->
-        ('a * 'b) FStar_Pervasives_Native.option
-  =
-  fun x ->
-    fun y ->
-      match (x, y) with
-      | (FStar_Pervasives_Native.Some x1, FStar_Pervasives_Native.Some y1) ->
-          FStar_Pervasives_Native.Some (x1, y1)
-      | uu___ -> FStar_Pervasives_Native.None
 let (find_field_string :
   Pollux_Proto_Descriptors.md ->
     Prims.string ->
@@ -172,19 +151,19 @@ let (find_tag : Pollux_Proto_Descriptors.pty -> tag) =
         -> LEN
     | Pollux_Proto_Descriptors.P_ENUM (Pollux_Proto_Descriptors.P_REPEATED)
         -> LEN
+    | Pollux_Proto_Descriptors.P_FIXED
+        (uu___, Pollux_Proto_Descriptors.P_REPEATED) -> LEN
+    | Pollux_Proto_Descriptors.P_SFIXED
+        (uu___, Pollux_Proto_Descriptors.P_REPEATED) -> LEN
+    | Pollux_Proto_Descriptors.P_FLOAT (Pollux_Proto_Descriptors.P_REPEATED)
+        -> LEN
+    | Pollux_Proto_Descriptors.P_DOUBLE (Pollux_Proto_Descriptors.P_REPEATED)
+        -> LEN
     | Pollux_Proto_Descriptors.P_INT (uu___, uu___1) -> VARINT
     | Pollux_Proto_Descriptors.P_UINT (uu___, uu___1) -> VARINT
     | Pollux_Proto_Descriptors.P_SINT (uu___, uu___1) -> VARINT
     | Pollux_Proto_Descriptors.P_BOOL uu___ -> VARINT
     | Pollux_Proto_Descriptors.P_ENUM uu___ -> VARINT
-    | Pollux_Proto_Descriptors.P_FIXED
-        (uu___, Pollux_Proto_Descriptors.P_REPEATED) when
-        uu___ = (Prims.of_int (32)) -> LEN
-    | Pollux_Proto_Descriptors.P_SFIXED
-        (uu___, Pollux_Proto_Descriptors.P_REPEATED) when
-        uu___ = (Prims.of_int (32)) -> LEN
-    | Pollux_Proto_Descriptors.P_FLOAT (Pollux_Proto_Descriptors.P_REPEATED)
-        -> LEN
     | Pollux_Proto_Descriptors.P_FIXED (uu___, uu___1) when
         uu___ = (Prims.of_int (32)) -> I32
     | Pollux_Proto_Descriptors.P_FIXED (uu___, uu___1) when
@@ -192,14 +171,6 @@ let (find_tag : Pollux_Proto_Descriptors.pty -> tag) =
     | Pollux_Proto_Descriptors.P_SFIXED (uu___, uu___1) when
         uu___ = (Prims.of_int (32)) -> I32
     | Pollux_Proto_Descriptors.P_FLOAT uu___ -> I32
-    | Pollux_Proto_Descriptors.P_FIXED
-        (uu___, Pollux_Proto_Descriptors.P_REPEATED) when
-        uu___ = (Prims.of_int (64)) -> I64
-    | Pollux_Proto_Descriptors.P_SFIXED
-        (uu___, Pollux_Proto_Descriptors.P_REPEATED) when
-        uu___ = (Prims.of_int (64)) -> I64
-    | Pollux_Proto_Descriptors.P_DOUBLE (Pollux_Proto_Descriptors.P_REPEATED)
-        -> I64
     | Pollux_Proto_Descriptors.P_FIXED (uu___, uu___1) when
         uu___ = (Prims.of_int (64)) -> I64
     | Pollux_Proto_Descriptors.P_SFIXED (uu___, uu___1) when
@@ -212,7 +183,7 @@ let (encode_header :
   =
   fun msg_d ->
     fun name ->
-      op_let_Question (find_field_string msg_d name)
+      Pollux_Proto_Prelude.op_let_Question (find_field_string msg_d name)
         (fun f ->
            let id_n =
              nat_to_u64
@@ -225,22 +196,34 @@ let (encode_header :
              (FStar_UInt64.logor
                 (FStar_UInt64.shift_left id_n (nat_to_u32 (Prims.of_int (3))))
                 tag_n))
-type bytes = FStar_UInt8.t Prims.list
-let (u64_of_s32 : FStar_Int32.t -> FStar_UInt64.t) =
-  fun s -> nat_to_u64 (sint_uint (Prims.of_int (32)) (FStar_Int32.v s))
-let (u64_of_s64 : FStar_Int64.t -> FStar_UInt64.t) =
-  fun s -> nat_to_u64 (sint_uint (Prims.of_int (64)) (FStar_Int64.v s))
-let (encode_int32 : FStar_Int32.t -> bytes) =
-  fun i -> Pollux_Proto_Varint.encode (FStar_Int_Cast.int32_to_uint64 i)
-let (encode_int64 : FStar_Int64.t -> bytes) =
-  fun i -> Pollux_Proto_Varint.encode (FStar_Int_Cast.int64_to_uint64 i)
-let (encode_uint32 : FStar_UInt32.t -> bytes) =
-  fun u -> Pollux_Proto_Varint.encode (FStar_Int_Cast.uint32_to_uint64 u)
-let (encode_sint32 : FStar_Int32.t -> bytes) =
+let (u64_of_s32 : Prims.int -> FStar_UInt64.t) =
+  fun s ->
+    nat_to_u64 (sint_uint (Prims.of_int (32)) (FStar_Int32.v (int_to_i32 s)))
+let (u64_of_s64 : Prims.int -> FStar_UInt64.t) =
+  fun s ->
+    nat_to_u64 (sint_uint (Prims.of_int (64)) (FStar_Int64.v (int_to_i64 s)))
+let (encode_int32 : Prims.int -> Pollux_Proto_Prelude.bytes) =
+  fun i ->
+    Pollux_Proto_Varint.encode
+      (FStar_Int_Cast.int64_to_uint64 (int_to_i64 i))
+let (encode_int64 : Prims.int -> Pollux_Proto_Prelude.bytes) =
+  fun i ->
+    Pollux_Proto_Varint.encode
+      (FStar_Int_Cast.int64_to_uint64 (int_to_i64 i))
+let (encode_uint32 : Prims.int -> Pollux_Proto_Prelude.bytes) =
+  fun u ->
+    Pollux_Proto_Varint.encode
+      (FStar_Int_Cast.int64_to_uint64 (int_to_i64 u))
+let (encode_uint64 : Prims.int -> Pollux_Proto_Prelude.bytes) =
+  fun u ->
+    Pollux_Proto_Varint.encode
+      (FStar_Int_Cast.int64_to_uint64 (int_to_i64 u))
+let (encode_sint32 : Prims.int -> Pollux_Proto_Prelude.bytes) =
   fun s -> Pollux_Proto_Varint.encode (u64_of_s32 s)
-let (encode_sint64 : FStar_Int64.t -> bytes) =
+let (encode_sint64 : Prims.int -> Pollux_Proto_Prelude.bytes) =
   fun s -> Pollux_Proto_Varint.encode (u64_of_s64 s)
-let rec (__encode_fixed32 : FStar_UInt32.t -> Prims.pos -> bytes) =
+let rec (__encode_fixed32 :
+  FStar_UInt32.t -> Prims.pos -> Pollux_Proto_Prelude.bytes) =
   fun x ->
     fun b ->
       let hi = FStar_UInt32.shift_right x (Stdint.Uint32.of_int (8)) in
@@ -250,9 +233,12 @@ let rec (__encode_fixed32 : FStar_UInt32.t -> Prims.pos -> bytes) =
       if b = Prims.int_one
       then [lo]
       else (let rx = __encode_fixed32 hi (b - Prims.int_one) in lo :: rx)
-let (encode_fixed32 : FStar_UInt32.t -> bytes) =
-  fun f -> __encode_fixed32 f (Prims.of_int (4))
-let rec (__encode_fixed64 : FStar_UInt64.t -> Prims.pos -> bytes) =
+let (encode_fixed32 : Prims.int -> Pollux_Proto_Prelude.bytes) =
+  fun f ->
+    __encode_fixed32 (FStar_Int_Cast.int32_to_uint32 (int_to_i32 f))
+      (Prims.of_int (4))
+let rec (__encode_fixed64 :
+  FStar_UInt64.t -> Prims.pos -> Pollux_Proto_Prelude.bytes) =
   fun x ->
     fun b ->
       let hi = FStar_UInt64.shift_right x (Stdint.Uint32.of_int (8)) in
@@ -262,32 +248,44 @@ let rec (__encode_fixed64 : FStar_UInt64.t -> Prims.pos -> bytes) =
       if b = Prims.int_one
       then [lo]
       else (let rx = __encode_fixed64 hi (b - Prims.int_one) in lo :: rx)
-let (encode_fixed64 : FStar_UInt64.t -> bytes) =
-  fun f -> __encode_fixed64 f (Prims.of_int (8))
-let (encode_sfixed32 : FStar_Int32.t -> bytes) =
-  fun i -> encode_fixed32 (FStar_Int_Cast.int32_to_uint32 i)
-let (encode_sfixed64 : FStar_Int64.t -> bytes) =
-  fun i -> encode_fixed64 (FStar_Int_Cast.int64_to_uint64 i)
-let (encode_bool : Prims.bool -> bytes) = fun b -> if b then [1] else [0]
+let (encode_fixed64 : Prims.int -> Pollux_Proto_Prelude.bytes) =
+  fun f ->
+    __encode_fixed64 (FStar_Int_Cast.int64_to_uint64 (int_to_i64 f))
+      (Prims.of_int (8))
+let (encode_sfixed32 : Prims.int -> Pollux_Proto_Prelude.bytes) =
+  fun i -> encode_fixed32 i
+let (encode_sfixed64 : Prims.int -> Pollux_Proto_Prelude.bytes) =
+  fun i -> encode_fixed64 i
+let (encode_bool : Prims.bool -> Pollux_Proto_Prelude.bytes) =
+  fun b -> if b then [1] else [0]
 let encode_implicit :
-  'a . 'a -> 'a -> ('a -> bytes) -> bytes FStar_Pervasives_Native.option =
+  'a .
+    'a ->
+      'a ->
+        ('a -> Pollux_Proto_Prelude.bytes) ->
+          Pollux_Proto_Prelude.bytes FStar_Pervasives_Native.option
+  =
   fun v ->
     fun d ->
       fun enc ->
         if v = d
         then FStar_Pervasives_Native.None
         else FStar_Pervasives_Native.Some (enc v)
-let encode_packed : 'a . 'a Prims.list -> ('a -> bytes) -> bytes =
+let encode_packed :
+  'a .
+    'a Prims.list ->
+      ('a -> Pollux_Proto_Prelude.bytes) -> Pollux_Proto_Prelude.bytes
+  =
   fun l ->
     fun enc_one ->
-      let bytes1 =
+      let bytes =
         FStar_List_Tot_Base.fold_left FStar_List_Tot_Base.append []
           (FStar_List_Tot_Base.map enc_one l) in
       let length =
         Pollux_Proto_Varint.encode
-          (nat_to_u64 (FStar_List_Tot_Base.length bytes1)) in
-      FStar_List_Tot_Base.op_At length bytes1
-let rec (encode_utf8_char : FStar_UInt32.t -> bytes) =
+          (nat_to_u64 (FStar_List_Tot_Base.length bytes)) in
+      FStar_List_Tot_Base.op_At length bytes
+let rec (encode_utf8_char : FStar_UInt32.t -> Pollux_Proto_Prelude.bytes) =
   fun x ->
     let hi = FStar_UInt32.shift_right x (Stdint.Uint32.of_int (8)) in
     let lo =
@@ -296,12 +294,13 @@ let rec (encode_utf8_char : FStar_UInt32.t -> bytes) =
     if FStar_UInt32.lte hi Stdint.Uint32.zero
     then [lo]
     else (let rx = encode_utf8_char hi in lo :: rx)
-let (encode_string : Prims.string -> bytes) =
+let (encode_string : Prims.string -> Pollux_Proto_Prelude.bytes) =
   fun s ->
     encode_packed
       (FStar_List_Tot_Base.map FStar_Char.u32_of_char
          (FStar_String.list_of_string s)) encode_utf8_char
-let (encode_bytes : bytes -> bytes) = fun b -> encode_packed b (fun x -> [x])
+let (encode_bytes : Pollux_Proto_Prelude.bytes -> Pollux_Proto_Prelude.bytes)
+  = fun b -> encode_packed b (fun x -> [x])
 let (v_measure : Pollux_Proto_Descriptors.vty -> Prims.nat) =
   fun v ->
     match v with
@@ -317,61 +316,7 @@ let (v_measure : Pollux_Proto_Descriptors.vty -> Prims.nat) =
          | Pollux_Proto_Descriptors.VOPTIONAL uu___ -> Prims.int_zero
          | Pollux_Proto_Descriptors.VREPEATED l ->
              FStar_List_Tot_Base.length l)
-    | Pollux_Proto_Descriptors.VINT32 v' ->
-        (match v' with
-         | Pollux_Proto_Descriptors.VIMPLICIT uu___ -> Prims.int_zero
-         | Pollux_Proto_Descriptors.VOPTIONAL uu___ -> Prims.int_zero
-         | Pollux_Proto_Descriptors.VREPEATED l ->
-             FStar_List_Tot_Base.length l)
-    | Pollux_Proto_Descriptors.VINT64 v' ->
-        (match v' with
-         | Pollux_Proto_Descriptors.VIMPLICIT uu___ -> Prims.int_zero
-         | Pollux_Proto_Descriptors.VOPTIONAL uu___ -> Prims.int_zero
-         | Pollux_Proto_Descriptors.VREPEATED l ->
-             FStar_List_Tot_Base.length l)
-    | Pollux_Proto_Descriptors.VUINT32 v' ->
-        (match v' with
-         | Pollux_Proto_Descriptors.VIMPLICIT uu___ -> Prims.int_zero
-         | Pollux_Proto_Descriptors.VOPTIONAL uu___ -> Prims.int_zero
-         | Pollux_Proto_Descriptors.VREPEATED l ->
-             FStar_List_Tot_Base.length l)
-    | Pollux_Proto_Descriptors.VUINT64 v' ->
-        (match v' with
-         | Pollux_Proto_Descriptors.VIMPLICIT uu___ -> Prims.int_zero
-         | Pollux_Proto_Descriptors.VOPTIONAL uu___ -> Prims.int_zero
-         | Pollux_Proto_Descriptors.VREPEATED l ->
-             FStar_List_Tot_Base.length l)
-    | Pollux_Proto_Descriptors.VSINT32 v' ->
-        (match v' with
-         | Pollux_Proto_Descriptors.VIMPLICIT uu___ -> Prims.int_zero
-         | Pollux_Proto_Descriptors.VOPTIONAL uu___ -> Prims.int_zero
-         | Pollux_Proto_Descriptors.VREPEATED l ->
-             FStar_List_Tot_Base.length l)
-    | Pollux_Proto_Descriptors.VSINT64 v' ->
-        (match v' with
-         | Pollux_Proto_Descriptors.VIMPLICIT uu___ -> Prims.int_zero
-         | Pollux_Proto_Descriptors.VOPTIONAL uu___ -> Prims.int_zero
-         | Pollux_Proto_Descriptors.VREPEATED l ->
-             FStar_List_Tot_Base.length l)
-    | Pollux_Proto_Descriptors.VFIXED32 v' ->
-        (match v' with
-         | Pollux_Proto_Descriptors.VIMPLICIT uu___ -> Prims.int_zero
-         | Pollux_Proto_Descriptors.VOPTIONAL uu___ -> Prims.int_zero
-         | Pollux_Proto_Descriptors.VREPEATED l ->
-             FStar_List_Tot_Base.length l)
-    | Pollux_Proto_Descriptors.VFIXED64 v' ->
-        (match v' with
-         | Pollux_Proto_Descriptors.VIMPLICIT uu___ -> Prims.int_zero
-         | Pollux_Proto_Descriptors.VOPTIONAL uu___ -> Prims.int_zero
-         | Pollux_Proto_Descriptors.VREPEATED l ->
-             FStar_List_Tot_Base.length l)
-    | Pollux_Proto_Descriptors.VSFIXED32 v' ->
-        (match v' with
-         | Pollux_Proto_Descriptors.VIMPLICIT uu___ -> Prims.int_zero
-         | Pollux_Proto_Descriptors.VOPTIONAL uu___ -> Prims.int_zero
-         | Pollux_Proto_Descriptors.VREPEATED l ->
-             FStar_List_Tot_Base.length l)
-    | Pollux_Proto_Descriptors.VSFIXED64 v' ->
+    | Pollux_Proto_Descriptors.VINT v' ->
         (match v' with
          | Pollux_Proto_Descriptors.VIMPLICIT uu___ -> Prims.int_zero
          | Pollux_Proto_Descriptors.VOPTIONAL uu___ -> Prims.int_zero
@@ -407,149 +352,102 @@ let (v_measure : Pollux_Proto_Descriptors.vty -> Prims.nat) =
          | Pollux_Proto_Descriptors.VOPTIONAL uu___ -> Prims.int_zero
          | Pollux_Proto_Descriptors.VREPEATED l ->
              FStar_List_Tot_Base.length l)
+let encode_dec_packed :
+  'a .
+    'a Pollux_Proto_Descriptors.dvty ->
+      'a ->
+        ('a -> Pollux_Proto_Prelude.bytes) ->
+          Pollux_Proto_Prelude.bytes FStar_Pervasives_Native.option
+  =
+  fun field ->
+    fun def ->
+      fun encode_one ->
+        match field with
+        | Pollux_Proto_Descriptors.VIMPLICIT v' ->
+            encode_implicit v' def encode_one
+        | Pollux_Proto_Descriptors.VOPTIONAL (FStar_Pervasives_Native.Some
+            v') -> FStar_Pervasives_Native.Some (encode_one v')
+        | Pollux_Proto_Descriptors.VREPEATED (vh::vt) ->
+            FStar_Pervasives_Native.Some
+              (encode_packed (vh :: vt) encode_one)
+        | uu___ -> FStar_Pervasives_Native.None
+let (find_encode_one :
+  Pollux_Proto_Descriptors.md ->
+    Prims.string ->
+      (Prims.int -> Pollux_Proto_Prelude.bytes)
+        FStar_Pervasives_Native.option)
+  =
+  fun msg_d ->
+    fun name ->
+      Pollux_Proto_Prelude.op_let_Question (find_field_string msg_d name)
+        (fun f ->
+           match FStar_Pervasives_Native.__proj__Mktuple3__item___3 f with
+           | Pollux_Proto_Descriptors.P_INT (uu___, uu___1) when
+               uu___ = (Prims.of_int (32)) ->
+               FStar_Pervasives_Native.Some encode_int32
+           | Pollux_Proto_Descriptors.P_INT (uu___, uu___1) when
+               uu___ = (Prims.of_int (64)) ->
+               FStar_Pervasives_Native.Some encode_int64
+           | Pollux_Proto_Descriptors.P_UINT (uu___, uu___1) when
+               uu___ = (Prims.of_int (32)) ->
+               FStar_Pervasives_Native.Some encode_uint32
+           | Pollux_Proto_Descriptors.P_UINT (uu___, uu___1) when
+               uu___ = (Prims.of_int (64)) ->
+               FStar_Pervasives_Native.Some encode_uint64
+           | Pollux_Proto_Descriptors.P_SINT (uu___, uu___1) when
+               uu___ = (Prims.of_int (32)) ->
+               FStar_Pervasives_Native.Some encode_sint32
+           | Pollux_Proto_Descriptors.P_SINT (uu___, uu___1) when
+               uu___ = (Prims.of_int (64)) ->
+               FStar_Pervasives_Native.Some encode_sint64
+           | Pollux_Proto_Descriptors.P_FIXED (uu___, uu___1) when
+               uu___ = (Prims.of_int (32)) ->
+               FStar_Pervasives_Native.Some encode_fixed32
+           | Pollux_Proto_Descriptors.P_FIXED (uu___, uu___1) when
+               uu___ = (Prims.of_int (64)) ->
+               FStar_Pervasives_Native.Some encode_fixed64
+           | Pollux_Proto_Descriptors.P_SFIXED (uu___, uu___1) when
+               uu___ = (Prims.of_int (32)) ->
+               FStar_Pervasives_Native.Some encode_sfixed32
+           | Pollux_Proto_Descriptors.P_SFIXED (uu___, uu___1) when
+               uu___ = (Prims.of_int (64)) ->
+               FStar_Pervasives_Native.Some encode_sfixed64
+           | uu___ -> FStar_Pervasives_Native.None)
 let rec (encode_field :
   Pollux_Proto_Descriptors.md ->
-    Pollux_Proto_Descriptors.vf -> bytes FStar_Pervasives_Native.option)
+    Pollux_Proto_Descriptors.vf ->
+      Pollux_Proto_Prelude.bytes FStar_Pervasives_Native.option)
   =
   fun msg_d ->
     fun field ->
-      op_let_Question
+      Pollux_Proto_Prelude.op_let_Question
         (encode_header msg_d
            (FStar_Pervasives_Native.__proj__Mktuple2__item___1 field))
         (fun header ->
            let header_bytes = Pollux_Proto_Varint.encode header in
-           op_let_Question (encode_value msg_d field)
+           Pollux_Proto_Prelude.op_let_Question (encode_value msg_d field)
              (fun value ->
                 FStar_Pervasives_Native.Some
                   (FStar_List_Tot_Base.op_At header_bytes value)))
 and (encode_value :
   Pollux_Proto_Descriptors.md ->
-    Pollux_Proto_Descriptors.vf -> bytes FStar_Pervasives_Native.option)
+    Pollux_Proto_Descriptors.vf ->
+      Pollux_Proto_Prelude.bytes FStar_Pervasives_Native.option)
   =
   fun msg_d ->
     fun field ->
       match FStar_Pervasives_Native.__proj__Mktuple2__item___2 field with
-      | Pollux_Proto_Descriptors.VDOUBLE (Pollux_Proto_Descriptors.VIMPLICIT
-          v') ->
-          encode_implicit v' Pollux_Proto_Descriptors.double_z (fun x -> x)
-      | Pollux_Proto_Descriptors.VDOUBLE (Pollux_Proto_Descriptors.VOPTIONAL
-          (FStar_Pervasives_Native.Some v')) ->
-          FStar_Pervasives_Native.Some v'
-      | Pollux_Proto_Descriptors.VDOUBLE (Pollux_Proto_Descriptors.VREPEATED
-          (vh::vt)) ->
-          FStar_Pervasives_Native.Some
-            (encode_packed (vh :: vt) (fun x -> x))
-      | Pollux_Proto_Descriptors.VFLOAT (Pollux_Proto_Descriptors.VIMPLICIT
-          v') ->
-          encode_implicit v' Pollux_Proto_Descriptors.float_z (fun x -> x)
-      | Pollux_Proto_Descriptors.VFLOAT (Pollux_Proto_Descriptors.VOPTIONAL
-          (FStar_Pervasives_Native.Some v')) ->
-          FStar_Pervasives_Native.Some v'
-      | Pollux_Proto_Descriptors.VFLOAT (Pollux_Proto_Descriptors.VREPEATED
-          (vh::vt)) ->
-          FStar_Pervasives_Native.Some
-            (encode_packed (vh :: vt) (fun x -> x))
-      | Pollux_Proto_Descriptors.VINT32 (Pollux_Proto_Descriptors.VIMPLICIT
-          v') -> encode_implicit v' Stdint.Int32.zero encode_int32
-      | Pollux_Proto_Descriptors.VINT32 (Pollux_Proto_Descriptors.VOPTIONAL
-          (FStar_Pervasives_Native.Some v')) ->
-          FStar_Pervasives_Native.Some (encode_int32 v')
-      | Pollux_Proto_Descriptors.VINT32 (Pollux_Proto_Descriptors.VREPEATED
-          (vh::vt)) ->
-          FStar_Pervasives_Native.Some
-            (encode_packed (vh :: vt) encode_int32)
-      | Pollux_Proto_Descriptors.VINT64 (Pollux_Proto_Descriptors.VIMPLICIT
-          v') -> encode_implicit v' Stdint.Int64.zero encode_int64
-      | Pollux_Proto_Descriptors.VINT64 (Pollux_Proto_Descriptors.VOPTIONAL
-          (FStar_Pervasives_Native.Some v')) ->
-          FStar_Pervasives_Native.Some (encode_int64 v')
-      | Pollux_Proto_Descriptors.VINT64 (Pollux_Proto_Descriptors.VREPEATED
-          (vh::vt)) ->
-          FStar_Pervasives_Native.Some
-            (encode_packed (vh :: vt) encode_int64)
-      | Pollux_Proto_Descriptors.VUINT32 (Pollux_Proto_Descriptors.VIMPLICIT
-          v') -> encode_implicit v' Stdint.Uint32.zero encode_uint32
-      | Pollux_Proto_Descriptors.VUINT32 (Pollux_Proto_Descriptors.VOPTIONAL
-          (FStar_Pervasives_Native.Some v')) ->
-          FStar_Pervasives_Native.Some (encode_uint32 v')
-      | Pollux_Proto_Descriptors.VUINT32 (Pollux_Proto_Descriptors.VREPEATED
-          (vh::vt)) ->
-          FStar_Pervasives_Native.Some
-            (encode_packed (vh :: vt) encode_uint32)
-      | Pollux_Proto_Descriptors.VUINT64 (Pollux_Proto_Descriptors.VIMPLICIT
-          v') ->
-          encode_implicit v' Stdint.Uint64.zero Pollux_Proto_Varint.encode
-      | Pollux_Proto_Descriptors.VUINT64 (Pollux_Proto_Descriptors.VOPTIONAL
-          (FStar_Pervasives_Native.Some v')) ->
-          FStar_Pervasives_Native.Some (Pollux_Proto_Varint.encode v')
-      | Pollux_Proto_Descriptors.VUINT64 (Pollux_Proto_Descriptors.VREPEATED
-          (vh::vt)) ->
-          FStar_Pervasives_Native.Some
-            (encode_packed (vh :: vt) Pollux_Proto_Varint.encode)
-      | Pollux_Proto_Descriptors.VSINT32 (Pollux_Proto_Descriptors.VIMPLICIT
-          v') -> encode_implicit v' Stdint.Int32.zero encode_sint32
-      | Pollux_Proto_Descriptors.VSINT32 (Pollux_Proto_Descriptors.VOPTIONAL
-          (FStar_Pervasives_Native.Some v')) ->
-          FStar_Pervasives_Native.Some (encode_sint32 v')
-      | Pollux_Proto_Descriptors.VSINT32 (Pollux_Proto_Descriptors.VREPEATED
-          (vh::vt)) ->
-          FStar_Pervasives_Native.Some
-            (encode_packed (vh :: vt) encode_sint32)
-      | Pollux_Proto_Descriptors.VSINT64 (Pollux_Proto_Descriptors.VIMPLICIT
-          v') -> encode_implicit v' Stdint.Int64.zero encode_sint64
-      | Pollux_Proto_Descriptors.VSINT64 (Pollux_Proto_Descriptors.VOPTIONAL
-          (FStar_Pervasives_Native.Some v')) ->
-          FStar_Pervasives_Native.Some (encode_sint64 v')
-      | Pollux_Proto_Descriptors.VSINT64 (Pollux_Proto_Descriptors.VREPEATED
-          (vh::vt)) ->
-          FStar_Pervasives_Native.Some
-            (encode_packed (vh :: vt) encode_sint64)
-      | Pollux_Proto_Descriptors.VFIXED32 (Pollux_Proto_Descriptors.VIMPLICIT
-          v') -> encode_implicit v' Stdint.Uint32.zero encode_fixed32
-      | Pollux_Proto_Descriptors.VFIXED32 (Pollux_Proto_Descriptors.VOPTIONAL
-          (FStar_Pervasives_Native.Some v')) ->
-          FStar_Pervasives_Native.Some (encode_fixed32 v')
-      | Pollux_Proto_Descriptors.VFIXED32 (Pollux_Proto_Descriptors.VREPEATED
-          (vh::vt)) ->
-          FStar_Pervasives_Native.Some
-            (encode_packed (vh :: vt) encode_fixed32)
-      | Pollux_Proto_Descriptors.VFIXED64 (Pollux_Proto_Descriptors.VIMPLICIT
-          v') -> encode_implicit v' Stdint.Uint64.zero encode_fixed64
-      | Pollux_Proto_Descriptors.VFIXED64 (Pollux_Proto_Descriptors.VOPTIONAL
-          (FStar_Pervasives_Native.Some v')) ->
-          FStar_Pervasives_Native.Some (encode_fixed64 v')
-      | Pollux_Proto_Descriptors.VFIXED64 (Pollux_Proto_Descriptors.VREPEATED
-          (vh::vt)) ->
-          FStar_Pervasives_Native.Some
-            (encode_packed (vh :: vt) encode_fixed64)
-      | Pollux_Proto_Descriptors.VSFIXED32
-          (Pollux_Proto_Descriptors.VIMPLICIT v') ->
-          encode_implicit v' Stdint.Int32.zero encode_sfixed32
-      | Pollux_Proto_Descriptors.VSFIXED32
-          (Pollux_Proto_Descriptors.VOPTIONAL (FStar_Pervasives_Native.Some
-          v')) -> FStar_Pervasives_Native.Some (encode_sfixed32 v')
-      | Pollux_Proto_Descriptors.VSFIXED32
-          (Pollux_Proto_Descriptors.VREPEATED (vh::vt)) ->
-          FStar_Pervasives_Native.Some
-            (encode_packed (vh :: vt) encode_sfixed32)
-      | Pollux_Proto_Descriptors.VSFIXED64
-          (Pollux_Proto_Descriptors.VIMPLICIT v') ->
-          encode_implicit v' Stdint.Int64.zero encode_sfixed64
-      | Pollux_Proto_Descriptors.VSFIXED64
-          (Pollux_Proto_Descriptors.VOPTIONAL (FStar_Pervasives_Native.Some
-          v')) -> FStar_Pervasives_Native.Some (encode_sfixed64 v')
-      | Pollux_Proto_Descriptors.VSFIXED64
-          (Pollux_Proto_Descriptors.VREPEATED (vh::vt)) ->
-          FStar_Pervasives_Native.Some
-            (encode_packed (vh :: vt) encode_sfixed64)
-      | Pollux_Proto_Descriptors.VBOOL (Pollux_Proto_Descriptors.VIMPLICIT
-          v') -> encode_implicit v' false encode_bool
-      | Pollux_Proto_Descriptors.VBOOL (Pollux_Proto_Descriptors.VOPTIONAL
-          (FStar_Pervasives_Native.Some v')) ->
-          FStar_Pervasives_Native.Some (encode_bool v')
-      | Pollux_Proto_Descriptors.VBOOL (Pollux_Proto_Descriptors.VREPEATED
-          (vh::vt)) ->
-          FStar_Pervasives_Native.Some (encode_packed (vh :: vt) encode_bool)
+      | Pollux_Proto_Descriptors.VDOUBLE v' ->
+          encode_dec_packed v' Pollux_Proto_Descriptors.double_z (fun x -> x)
+      | Pollux_Proto_Descriptors.VFLOAT v' ->
+          encode_dec_packed v' Pollux_Proto_Descriptors.float_z (fun x -> x)
+      | Pollux_Proto_Descriptors.VINT v' ->
+          Pollux_Proto_Prelude.op_let_Question
+            (find_encode_one msg_d
+               (FStar_Pervasives_Native.__proj__Mktuple2__item___1 field))
+            (fun encode_one -> encode_dec_packed v' Prims.int_zero encode_one)
+      | Pollux_Proto_Descriptors.VBOOL v' ->
+          encode_dec_packed v' false encode_bool
       | Pollux_Proto_Descriptors.VSTRING (Pollux_Proto_Descriptors.VIMPLICIT
           v') -> encode_implicit v' "" encode_string
       | Pollux_Proto_Descriptors.VSTRING (Pollux_Proto_Descriptors.VOPTIONAL
@@ -602,9 +500,482 @@ let opt_append :
       | FStar_Pervasives_Native.None -> l1
       | FStar_Pervasives_Native.Some l2' -> FStar_List_Tot_Base.op_At l1 l2'
 let (encode_message :
-  Pollux_Proto_Descriptors.md -> Pollux_Proto_Descriptors.msg -> bytes) =
+  Pollux_Proto_Descriptors.md ->
+    Pollux_Proto_Descriptors.msg -> Pollux_Proto_Prelude.bytes)
+  =
   fun md ->
     fun msg ->
       let encoder = encode_field md in
       FStar_List_Tot_Base.fold_left opt_append []
         (FStar_List_Tot_Base.map encoder msg)
+let (tag_from_num : FStar_UInt64.t -> tag FStar_Pervasives_Native.option) =
+  fun n ->
+    match n with
+    | uu___ when uu___ = Stdint.Uint64.zero ->
+        FStar_Pervasives_Native.Some VARINT
+    | uu___ when uu___ = Stdint.Uint64.one ->
+        FStar_Pervasives_Native.Some I64
+    | uu___ when uu___ = (Stdint.Uint64.of_int (2)) ->
+        FStar_Pervasives_Native.Some LEN
+    | uu___ when uu___ = (Stdint.Uint64.of_int (5)) ->
+        FStar_Pervasives_Native.Some I32
+    | uu___ -> FStar_Pervasives_Native.None
+let (decode_header :
+  Pollux_Proto_Prelude.bytes ->
+    (Prims.nat * tag * Pollux_Proto_Prelude.bytes)
+      FStar_Pervasives_Native.option)
+  =
+  fun enc ->
+    Pollux_Proto_Prelude.op_let_Question
+      (Pollux_Proto_Varint.extract_varint enc)
+      (fun uu___ ->
+         match uu___ with
+         | (header_bytes, bs) ->
+             let header = Pollux_Proto_Varint.decode header_bytes in
+             let fid =
+               FStar_UInt64.v
+                 (FStar_UInt64.shift_right header (Stdint.Uint32.of_int (3))) in
+             let tag_n =
+               FStar_UInt64.logand header (Stdint.Uint64.of_int (7)) in
+             Pollux_Proto_Prelude.op_let_Question (tag_from_num tag_n)
+               (fun tag1 -> FStar_Pervasives_Native.Some (fid, tag1, bs)))
+let (find_field :
+  Pollux_Proto_Descriptors.md ->
+    Prims.nat -> Pollux_Proto_Descriptors.fd FStar_Pervasives_Native.option)
+  =
+  fun md ->
+    fun id ->
+      FStar_List_Tot_Base.find
+        (fun f -> (FStar_Pervasives_Native.__proj__Mktuple3__item___2 f) = id)
+        md.Pollux_Proto_Descriptors.fields
+let rec take :
+  'a .
+    Prims.nat ->
+      'a Prims.list ->
+        ('a Prims.list * 'a Prims.list) FStar_Pervasives_Native.option
+  =
+  fun n ->
+    fun l ->
+      if n = Prims.int_zero
+      then FStar_Pervasives_Native.Some ([], l)
+      else
+        (match l with
+         | [] -> FStar_Pervasives_Native.None
+         | hd::tl ->
+             Pollux_Proto_Prelude.op_let_Question
+               (take (n - Prims.int_one) tl)
+               (fun uu___1 ->
+                  match uu___1 with
+                  | (l1, l2) -> FStar_Pervasives_Native.Some ((hd :: l1), l2)))
+let (decode_value :
+  tag ->
+    Pollux_Proto_Prelude.bytes ->
+      (Pollux_Proto_Prelude.bytes * Pollux_Proto_Prelude.bytes)
+        FStar_Pervasives_Native.option)
+  =
+  fun t ->
+    fun enc ->
+      match t with
+      | VARINT ->
+          Pollux_Proto_Prelude.op_let_Question
+            (Pollux_Proto_Varint.extract_varint enc)
+            (fun v ->
+               let vint =
+                 FStar_Pervasives_Native.__proj__Mktuple2__item___1 v in
+               let byt = FStar_Pervasives_Native.__proj__Mktuple2__item___2 v in
+               FStar_Pervasives_Native.Some (vint, byt))
+      | I64 ->
+          (match take (Prims.of_int (8)) enc with
+           | FStar_Pervasives_Native.None -> FStar_Pervasives_Native.None
+           | FStar_Pervasives_Native.Some (i64, b) ->
+               FStar_Pervasives_Native.Some (i64, b))
+      | LEN ->
+          Pollux_Proto_Prelude.op_let_Question
+            (Pollux_Proto_Varint.extract_varint enc)
+            (fun uu___ ->
+               match uu___ with
+               | (len_byt, enc_byt) ->
+                   let len = Pollux_Proto_Varint.decode len_byt in
+                   if FStar_UInt64.eq len Stdint.Uint64.zero
+                   then FStar_Pervasives_Native.Some ([], enc_byt)
+                   else
+                     (match take (FStar_UInt64.v len) enc_byt with
+                      | FStar_Pervasives_Native.None ->
+                          FStar_Pervasives_Native.None
+                      | FStar_Pervasives_Native.Some tak ->
+                          let len_byt1 = FStar_Pervasives_Native.fst tak in
+                          let rest_byt = FStar_Pervasives_Native.snd tak in
+                          FStar_Pervasives_Native.Some (len_byt1, rest_byt)))
+      | I32 ->
+          (match take (Prims.of_int (4)) enc with
+           | FStar_Pervasives_Native.None -> FStar_Pervasives_Native.None
+           | FStar_Pervasives_Native.Some (i32, b) ->
+               FStar_Pervasives_Native.Some (i32, b))
+      | uu___ -> FStar_Pervasives_Native.None
+let (decode_field :
+  Pollux_Proto_Prelude.bytes ->
+    (Prims.nat * Pollux_Proto_Prelude.bytes * Pollux_Proto_Prelude.bytes)
+      FStar_Pervasives_Native.option)
+  =
+  fun enc ->
+    match decode_header enc with
+    | FStar_Pervasives_Native.None -> FStar_Pervasives_Native.None
+    | FStar_Pervasives_Native.Some (fid, t, bs) ->
+        (match decode_value t bs with
+         | FStar_Pervasives_Native.None -> FStar_Pervasives_Native.None
+         | FStar_Pervasives_Native.Some (v, b) ->
+             FStar_Pervasives_Native.Some (fid, v, b))
+let rec (decode_fields :
+  Pollux_Proto_Prelude.bytes ->
+    ((Prims.nat * Pollux_Proto_Prelude.bytes) Prims.list *
+      Pollux_Proto_Prelude.bytes))
+  =
+  fun enc ->
+    match enc with
+    | [] -> ([], [])
+    | enc1 ->
+        (match decode_field enc1 with
+         | FStar_Pervasives_Native.None -> ([], enc1)
+         | FStar_Pervasives_Native.Some (fid, fbs, bs) ->
+             let uu___ = decode_fields bs in
+             (match uu___ with
+              | (rest_fields, rest_byt) ->
+                  (((fid, fbs) :: rest_fields), rest_byt)))
+type 'a field_parser =
+  Pollux_Proto_Prelude.bytes ->
+    ('a * Pollux_Proto_Prelude.bytes) FStar_Pervasives_Native.option
+let rec (assemble_nat : Pollux_Proto_Prelude.bytes -> Prims.nat) =
+  fun b ->
+    match b with
+    | [] -> Prims.int_zero
+    | hd::tl ->
+        let rest = (Prims.pow2 (Prims.of_int (8))) * (assemble_nat tl) in
+        (FStar_UInt8.v hd) + rest
+let (parse_double : Pollux_Proto_Descriptors.double field_parser) =
+  fun b ->
+    match take (Prims.of_int (8)) b with
+    | FStar_Pervasives_Native.None -> FStar_Pervasives_Native.None
+    | FStar_Pervasives_Native.Some db ->
+        FStar_Pervasives_Native.Some
+          ((FStar_Pervasives_Native.fst db),
+            (FStar_Pervasives_Native.snd db))
+let (parse_float : Pollux_Proto_Descriptors.float field_parser) =
+  fun b ->
+    match take (Prims.of_int (4)) b with
+    | FStar_Pervasives_Native.None -> FStar_Pervasives_Native.None
+    | FStar_Pervasives_Native.Some db ->
+        FStar_Pervasives_Native.Some
+          ((FStar_Pervasives_Native.fst db),
+            (FStar_Pervasives_Native.snd db))
+let (parse_int : Pollux_Proto_Descriptors.width -> Prims.int field_parser) =
+  fun w ->
+    fun b ->
+      match Pollux_Proto_Varint.extract_varint b with
+      | FStar_Pervasives_Native.None -> FStar_Pervasives_Native.None
+      | FStar_Pervasives_Native.Some vint ->
+          let raw_v =
+            FStar_UInt64.v
+              (Pollux_Proto_Varint.decode (FStar_Pervasives_Native.fst vint)) in
+          let v = uint_int w (uint_change_w w raw_v) in
+          FStar_Pervasives_Native.Some
+            (v, (FStar_Pervasives_Native.snd vint))
+let (parse_uint : Pollux_Proto_Descriptors.width -> Prims.int field_parser) =
+  fun w ->
+    fun b ->
+      match Pollux_Proto_Varint.extract_varint b with
+      | FStar_Pervasives_Native.None -> FStar_Pervasives_Native.None
+      | FStar_Pervasives_Native.Some vint ->
+          let raw_v =
+            FStar_UInt64.v
+              (Pollux_Proto_Varint.decode (FStar_Pervasives_Native.fst vint)) in
+          let v = uint_change_w w raw_v in
+          FStar_Pervasives_Native.Some
+            (v, (FStar_Pervasives_Native.snd vint))
+let (parse_sint : Pollux_Proto_Descriptors.width -> Prims.int field_parser) =
+  fun w ->
+    fun b ->
+      match Pollux_Proto_Varint.extract_varint b with
+      | FStar_Pervasives_Native.None -> FStar_Pervasives_Native.None
+      | FStar_Pervasives_Native.Some vint ->
+          let raw_v =
+            FStar_UInt64.v
+              (Pollux_Proto_Varint.decode (FStar_Pervasives_Native.fst vint)) in
+          let v = uint_sint w (uint_change_w w raw_v) in
+          FStar_Pervasives_Native.Some
+            (v, (FStar_Pervasives_Native.snd vint))
+let (parse_fixed : Pollux_Proto_Descriptors.width -> Prims.int field_parser)
+  =
+  fun w ->
+    fun b ->
+      let n = w / (Prims.of_int (8)) in
+      match take n b with
+      | FStar_Pervasives_Native.None -> FStar_Pervasives_Native.None
+      | FStar_Pervasives_Native.Some db ->
+          FStar_Pervasives_Native.Some
+            ((assemble_nat (FStar_Pervasives_Native.fst db)),
+              (FStar_Pervasives_Native.snd db))
+let (parse_sfixed : Pollux_Proto_Descriptors.width -> Prims.int field_parser)
+  =
+  fun w ->
+    fun b ->
+      let n = w / (Prims.of_int (8)) in
+      match take n b with
+      | FStar_Pervasives_Native.None -> FStar_Pervasives_Native.None
+      | FStar_Pervasives_Native.Some db ->
+          FStar_Pervasives_Native.Some
+            ((uint_int w (assemble_nat (FStar_Pervasives_Native.fst db))),
+              (FStar_Pervasives_Native.snd db))
+let (parse_bool : Prims.bool field_parser) =
+  fun b ->
+    match b with
+    | uu___::tl when uu___ = 0 -> FStar_Pervasives_Native.Some (false, tl)
+    | uu___::tl when uu___ = 1 -> FStar_Pervasives_Native.Some (true, tl)
+    | uu___ -> FStar_Pervasives_Native.None
+let (parse_string : Prims.string field_parser) =
+  fun b ->
+    if FStar_List_Tot_Base.isEmpty b
+    then FStar_Pervasives_Native.None
+    else
+      (let s =
+         FStar_String.string_of_list
+           (FStar_List_Tot_Base.map
+              (fun b1 -> FStar_Char.char_of_int (FStar_UInt8.v b1)) b) in
+       FStar_Pervasives_Native.Some (s, []))
+let (parse_bytes : Pollux_Proto_Prelude.bytes field_parser) =
+  fun b ->
+    if FStar_List_Tot_Base.isEmpty b
+    then FStar_Pervasives_Native.None
+    else FStar_Pervasives_Native.Some (b, [])
+let rec parse_list :
+  'a .
+    Pollux_Proto_Prelude.bytes ->
+      'a field_parser -> 'a Prims.list FStar_Pervasives_Native.option
+  =
+  fun payload ->
+    fun parse_one ->
+      match parse_one payload with
+      | FStar_Pervasives_Native.None -> FStar_Pervasives_Native.None
+      | FStar_Pervasives_Native.Some (a1, bs) ->
+          if FStar_List_Tot_Base.isEmpty bs
+          then FStar_Pervasives_Native.Some [a1]
+          else
+            (let rest = parse_list bs parse_one in
+             match rest with
+             | FStar_Pervasives_Native.None -> FStar_Pervasives_Native.None
+             | FStar_Pervasives_Native.Some r ->
+                 FStar_Pervasives_Native.Some (a1 :: r))
+let parse_dec :
+  'a .
+    Pollux_Proto_Descriptors.pdec ->
+      Pollux_Proto_Prelude.bytes ->
+        'a field_parser ->
+          'a Pollux_Proto_Descriptors.dvty FStar_Pervasives_Native.option
+  =
+  fun dec ->
+    fun payload ->
+      fun parse_one ->
+        match dec with
+        | Pollux_Proto_Descriptors.P_IMPLICIT ->
+            Pollux_Proto_Prelude.op_let_Question (parse_one payload)
+              (fun uu___ ->
+                 match uu___ with
+                 | (one, uu___1) ->
+                     FStar_Pervasives_Native.Some
+                       (Pollux_Proto_Descriptors.VIMPLICIT one))
+        | Pollux_Proto_Descriptors.P_OPTIONAL ->
+            Pollux_Proto_Prelude.op_let_Question (parse_one payload)
+              (fun uu___ ->
+                 match uu___ with
+                 | (one, uu___1) ->
+                     FStar_Pervasives_Native.Some
+                       (Pollux_Proto_Descriptors.VOPTIONAL
+                          (FStar_Pervasives_Native.Some one)))
+        | Pollux_Proto_Descriptors.P_REPEATED ->
+            Pollux_Proto_Prelude.op_let_Question
+              (parse_list payload parse_one)
+              (fun many ->
+                 FStar_Pervasives_Native.Some
+                   (Pollux_Proto_Descriptors.VREPEATED many))
+let (parse_field :
+  Pollux_Proto_Descriptors.pty ->
+    Pollux_Proto_Prelude.bytes ->
+      Pollux_Proto_Descriptors.vty FStar_Pervasives_Native.option)
+  =
+  fun ty ->
+    fun payload ->
+      match ty with
+      | Pollux_Proto_Descriptors.P_DOUBLE p' ->
+          Pollux_Proto_Prelude.op_let_Question
+            (parse_dec p' payload parse_double)
+            (fun vdec ->
+               FStar_Pervasives_Native.Some
+                 (Pollux_Proto_Descriptors.VDOUBLE vdec))
+      | Pollux_Proto_Descriptors.P_FLOAT p' ->
+          Pollux_Proto_Prelude.op_let_Question
+            (parse_dec p' payload parse_float)
+            (fun vdec ->
+               FStar_Pervasives_Native.Some
+                 (Pollux_Proto_Descriptors.VFLOAT vdec))
+      | Pollux_Proto_Descriptors.P_INT (w, p') ->
+          Pollux_Proto_Prelude.op_let_Question
+            (parse_dec p' payload (parse_int w))
+            (fun vdec ->
+               FStar_Pervasives_Native.Some
+                 (Pollux_Proto_Descriptors.VINT vdec))
+      | Pollux_Proto_Descriptors.P_UINT (w, p') ->
+          Pollux_Proto_Prelude.op_let_Question
+            (parse_dec p' payload (parse_uint w))
+            (fun vdec ->
+               FStar_Pervasives_Native.Some
+                 (Pollux_Proto_Descriptors.VINT vdec))
+      | Pollux_Proto_Descriptors.P_SINT (w, p') ->
+          Pollux_Proto_Prelude.op_let_Question
+            (parse_dec p' payload (parse_sint w))
+            (fun vdec ->
+               FStar_Pervasives_Native.Some
+                 (Pollux_Proto_Descriptors.VINT vdec))
+      | Pollux_Proto_Descriptors.P_FIXED (w, p') ->
+          Pollux_Proto_Prelude.op_let_Question
+            (parse_dec p' payload (parse_fixed w))
+            (fun vdec ->
+               FStar_Pervasives_Native.Some
+                 (Pollux_Proto_Descriptors.VINT vdec))
+      | Pollux_Proto_Descriptors.P_SFIXED (w, p') ->
+          Pollux_Proto_Prelude.op_let_Question
+            (parse_dec p' payload (parse_sfixed w))
+            (fun vdec ->
+               FStar_Pervasives_Native.Some
+                 (Pollux_Proto_Descriptors.VINT vdec))
+      | Pollux_Proto_Descriptors.P_BOOL p' ->
+          Pollux_Proto_Prelude.op_let_Question
+            (parse_dec p' payload parse_bool)
+            (fun vdec ->
+               FStar_Pervasives_Native.Some
+                 (Pollux_Proto_Descriptors.VBOOL vdec))
+      | Pollux_Proto_Descriptors.P_STRING p' ->
+          Pollux_Proto_Prelude.op_let_Question
+            (parse_dec p' payload parse_string)
+            (fun vdec ->
+               FStar_Pervasives_Native.Some
+                 (Pollux_Proto_Descriptors.VSTRING vdec))
+      | Pollux_Proto_Descriptors.P_BYTES p' ->
+          Pollux_Proto_Prelude.op_let_Question
+            (parse_dec p' payload parse_bytes)
+            (fun vdec ->
+               FStar_Pervasives_Native.Some
+                 (Pollux_Proto_Descriptors.VBYTES vdec))
+      | uu___ -> FStar_Pervasives_Native.None
+let update_field :
+  'a .
+    Prims.string ->
+      'a Pollux_Proto_Descriptors.dvty ->
+        'a Pollux_Proto_Descriptors.dvty -> 'a Pollux_Proto_Descriptors.dvty
+  =
+  fun name ->
+    fun ori_v ->
+      fun new_v ->
+        match (ori_v, new_v) with
+        | (Pollux_Proto_Descriptors.VIMPLICIT uu___,
+           Pollux_Proto_Descriptors.VIMPLICIT v') ->
+            Pollux_Proto_Descriptors.VIMPLICIT v'
+        | (Pollux_Proto_Descriptors.VOPTIONAL uu___,
+           Pollux_Proto_Descriptors.VOPTIONAL v') ->
+            Pollux_Proto_Descriptors.VOPTIONAL v'
+        | (Pollux_Proto_Descriptors.VREPEATED v',
+           Pollux_Proto_Descriptors.VREPEATED value') ->
+            Pollux_Proto_Descriptors.VREPEATED
+              (FStar_List_Tot_Base.op_At v' value')
+        | uu___ -> ori_v
+let rec (update_msg :
+  Pollux_Proto_Descriptors.msg ->
+    Prims.string ->
+      Pollux_Proto_Descriptors.vty -> Pollux_Proto_Descriptors.msg)
+  =
+  fun msg ->
+    fun name ->
+      fun value ->
+        match msg with
+        | [] -> []
+        | hd::tl ->
+            let n = FStar_Pervasives_Native.fst hd in
+            let v = FStar_Pervasives_Native.snd hd in
+            if n = name
+            then
+              (n,
+                ((match (v, value) with
+                  | (Pollux_Proto_Descriptors.VDOUBLE orig,
+                     Pollux_Proto_Descriptors.VDOUBLE newv) ->
+                      Pollux_Proto_Descriptors.VDOUBLE
+                        (update_field n orig newv)
+                  | (Pollux_Proto_Descriptors.VFLOAT orig,
+                     Pollux_Proto_Descriptors.VFLOAT newv) ->
+                      Pollux_Proto_Descriptors.VFLOAT
+                        (update_field n orig newv)
+                  | (Pollux_Proto_Descriptors.VINT orig,
+                     Pollux_Proto_Descriptors.VINT newv) ->
+                      Pollux_Proto_Descriptors.VINT
+                        (update_field n orig newv)
+                  | (Pollux_Proto_Descriptors.VBOOL orig,
+                     Pollux_Proto_Descriptors.VBOOL newv) ->
+                      Pollux_Proto_Descriptors.VBOOL
+                        (update_field n orig newv)
+                  | (Pollux_Proto_Descriptors.VSTRING orig,
+                     Pollux_Proto_Descriptors.VSTRING newv) ->
+                      Pollux_Proto_Descriptors.VSTRING
+                        (update_field n orig newv)
+                  | (Pollux_Proto_Descriptors.VBYTES orig,
+                     Pollux_Proto_Descriptors.VBYTES newv) ->
+                      Pollux_Proto_Descriptors.VBYTES
+                        (update_field n orig newv)
+                  | (Pollux_Proto_Descriptors.VMSG orig,
+                     Pollux_Proto_Descriptors.VMSG newv) ->
+                      Pollux_Proto_Descriptors.VMSG
+                        (update_field n orig newv)
+                  | (Pollux_Proto_Descriptors.VENUM orig,
+                     Pollux_Proto_Descriptors.VENUM newv) ->
+                      Pollux_Proto_Descriptors.VENUM
+                        (update_field n orig newv)
+                  | uu___ -> v)))
+              :: tl
+            else (let r = update_msg tl name value in hd :: r)
+let (merge_field :
+  Pollux_Proto_Descriptors.md ->
+    Pollux_Proto_Descriptors.msg FStar_Pervasives_Native.option ->
+      (Prims.nat * Pollux_Proto_Prelude.bytes) ->
+        Pollux_Proto_Descriptors.msg FStar_Pervasives_Native.option)
+  =
+  fun m ->
+    fun msg ->
+      fun f ->
+        Pollux_Proto_Prelude.op_let_Question msg
+          (fun msg1 ->
+             let uu___ = f in
+             match uu___ with
+             | (fid, payload) ->
+                 let field_desc = find_field m fid in
+                 (match field_desc with
+                  | FStar_Pervasives_Native.None ->
+                      FStar_Pervasives_Native.Some msg1
+                  | FStar_Pervasives_Native.Some (n, f1, ty) ->
+                      Pollux_Proto_Prelude.op_let_Question
+                        (parse_field ty payload)
+                        (fun typed_payload ->
+                           let new_msg = update_msg msg1 n typed_payload in
+                           FStar_Pervasives_Native.Some new_msg)))
+let (parse :
+  Pollux_Proto_Descriptors.md ->
+    Pollux_Proto_Prelude.bytes ->
+      Pollux_Proto_Descriptors.msg FStar_Pervasives_Native.option)
+  =
+  fun m ->
+    fun enc ->
+      let uu___ = decode_fields enc in
+      match uu___ with
+      | (raw_fields, leftover_byt) ->
+          if leftover_byt <> []
+          then FStar_Pervasives_Native.None
+          else
+            (let msg = Pollux_Proto_Descriptors.init_msg m in
+             let field_merge = merge_field m in
+             FStar_List_Tot_Base.fold_left field_merge
+               (FStar_Pervasives_Native.Some msg) raw_fields)
