pollux/lib/pollux/Pollux_Proto_Prelude.ml
@@ -1,0 +1,25 @@
+open Prims
+type bytes = FStar_UInt8.t Prims.list
+let op_let_Question :
+  'a 'b .
+    'a FStar_Pervasives_Native.option ->
+      ('a -> 'b FStar_Pervasives_Native.option) ->
+        'b FStar_Pervasives_Native.option
+  =
+  fun x ->
+    fun f ->
+      match x with
+      | FStar_Pervasives_Native.Some x1 -> f x1
+      | FStar_Pervasives_Native.None -> FStar_Pervasives_Native.None
+let op_and_Question :
+  'a 'b .
+    'a FStar_Pervasives_Native.option ->
+      'b FStar_Pervasives_Native.option ->
+        ('a * 'b) FStar_Pervasives_Native.option
+  =
+  fun x ->
+    fun y ->
+      match (x, y) with
+      | (FStar_Pervasives_Native.Some x1, FStar_Pervasives_Native.Some y1) ->
+          FStar_Pervasives_Native.Some (x1, y1)
+      | uu___ -> FStar_Pervasives_Native.None
